Table/BuiltinExtensions/List/Basic.lean
@@ -1,0 +1,228 @@
+import Table.BuiltinExtensions.List.Predicates
+import Table.BuiltinExtensions.Numeric
+
+/-!
+Basic list functions and lemmas.
+-/
+
+def List.certifiedMap {α β} :
+  (xs : List α) → ((x : α) → List.MemT x xs → β) → List β
+| [], f => []
+| x :: xs, f =>
+  f x (MemT.hd x xs) :: certifiedMap xs (λ x' pf => f x' $ MemT.tl _ pf)
+
+def List.prod {α β} : List α → List β → List (α × β)
+| [], _ => []
+| _, [] => []
+| [x], y :: ys => (x, y) :: prod [x] ys
+| x :: x' :: xs, ys =>
+  have h₁ : Nat.succ 0 + length ys <
+            Nat.succ (Nat.succ (length xs)) + length ys :=
+    by apply Nat.add_lt_add_right
+       apply Nat.succ_lt_succ $ Nat.succ_pos (length xs)
+  have h₂ : Nat.succ (length xs) + length ys <
+            Nat.succ (Nat.succ (length xs)) + length ys :=
+    by apply Nat.add_lt_add_right
+       apply Nat.succ_lt_succ
+       apply Nat.lt.base
+  prod [x] ys ++ prod (x' :: xs) ys
+termination_by xs ys => xs.length + ys.length
+
+def List.dropLastN {α} : Nat → List α → List α :=
+  (λ n => reverse ∘ List.drop n ∘ reverse)
+
+def List.flatten {α} : List (List α) → List α
+| [] => []
+| [] :: ys => flatten ys
+| (x :: xs) :: ys => x :: flatten (xs :: ys)
+
+def List.sum : List Nat → Nat
+| [] => 0
+| x :: xs => x + sum xs
+
+def List.toSingletons : List α → List (List α)
+| [] => []
+| x :: xs => [x] :: toSingletons xs
+
+def List.somes : List (Option α) → List α
+| [] => []
+| none :: xs => somes xs
+| some x :: xs => x :: somes xs
+
+-- From a failed approach to `pivotTable` -- keeping around just in case
+def List.depFoldr {κ : List α → Type _} :
+  (xs : List α) →
+  (∀ {xs : List α} (x : α), κ xs → κ (x :: xs)) →
+  κ [] →
+  κ xs
+| [], f, z => z
+| x :: xs, f, z => f x (depFoldr xs f z)
+
+def List.memT_somes_of_memT {α} : ∀ {x : α} {xs : List (Option α)},
+  List.MemT (some x) xs → List.MemT x xs.somes
+| x, .(some x) :: xs, .hd .(some x) .(xs) => .hd x xs.somes
+| x, (some y) :: xs, .tl .(some y) htl => .tl y $ memT_somes_of_memT htl
+| x, none :: xs, .tl _ htl => @memT_somes_of_memT α x xs htl
+
+def List.memT_map_of_memT {α β} (f : α → β) {x : α} :
+  ∀ {xs : List α}, MemT x xs → MemT (f x) (map f xs)
+| .(x) :: xs, .hd _ _ => .hd _ _
+| _ :: xs, .tl _ htl => .tl _ <| memT_map_of_memT _ htl
+
+def List.vEnumFrom (xs : List α) :
+  (n : Nat) → (ys : List α) → (n + ys.length ≤ xs.length) →
+  List (Fin xs.length × α)
+| n, [], _ => []
+| n, y :: ys, pf =>
+  (⟨n, Nat.lt_of_lt_add_left pf⟩, y) ::
+  vEnumFrom xs (n + 1) ys (Eq.subst (motive := (· ≤ length xs))
+                  (Nat.add_right_comm n (length ys) 1) pf)
+
+def List.verifiedEnum (xs : List α) : List (Fin xs.length × α) :=
+  vEnumFrom xs 0 xs (Eq.subst (Nat.zero_add _) (Nat.le_refl _))
+
+theorem List.length_vEnumFrom (xs : List α) :
+  ∀ (ys : List α) (n : Nat) (pf : n + ys.length ≤ xs.length),
+  (vEnumFrom xs n ys pf).length = ys.length
+| [], _, _ => rfl
+| y :: ys, n, pf => congrArg (·+1) (length_vEnumFrom xs ys (n + 1) _)
+
+theorem List.length_verifiedEnum : ∀ (xs : List α),
+  xs.verifiedEnum.length = xs.length
+| [] => rfl
+| x :: xs => congrArg (·+1) (length_vEnumFrom _ _ _ _)
+
+theorem List.zip_length_eq_of_length_eq :
+  ∀ (xs : List α) (ys : List β) (h : xs.length = ys.length),
+    (List.zip xs ys).length = xs.length
+| [], [], _ => rfl
+| (x :: xs), (y :: ys), h =>
+  have ih := zip_length_eq_of_length_eq xs ys (by
+    simp only [List.length] at h
+    apply Nat.succ.inj
+    apply h
+  )
+  congrArg (λ x => x + 1) ih
+
+theorem List.length_prod : ∀ (xs : List α) (ys : List β),
+  List.length (List.prod xs ys) = xs.length * ys.length
+| [], _ => by simp [prod, length]
+| x :: xs, [] => by simp [prod, length]
+| [x], y :: ys =>
+  have ih := length_prod [x] ys
+  by simp only [prod]
+     unfold length  -- adding `length` to the simp above does bad things
+     rw [ih]
+     simp only [length]
+     rw [Nat.one_mul, Nat.one_mul]
+| x :: x' :: xs, y :: ys =>
+  have h_term₁ : Nat.succ 0 + Nat.succ (length ys) <
+                 Nat.succ (Nat.succ (length xs)) + Nat.succ (length ys) :=
+    by apply Nat.add_lt_add_right
+       apply Nat.succ_lt_succ $ Nat.succ_pos (length xs)
+  have h_term₂ : Nat.succ (length xs) + Nat.succ (length ys) <
+                 Nat.succ (Nat.succ (length xs)) + Nat.succ (length ys) :=
+    by apply Nat.add_lt_add_right
+       apply Nat.succ_lt_succ
+       apply Nat.lt.base
+  have ih₁ := length_prod [x] (y :: ys)
+  have ih₂ := length_prod (x' :: xs) (y :: ys)
+  by unfold prod
+     simp only
+     rw [List.length_append, ih₁, ih₂]
+     simp only [length]
+     rw [←Nat.add_mul, Nat.zero_add, Nat.add_comm 1]
+termination_by xs ys => xs.length + ys.length
+
+theorem List.length_take_of_lt :
+  ∀ (n : Nat) (xs : List α) (h : n < xs.length),
+    length (List.take n xs) = n
+| _, [], h => by cases h
+| 0, _, _ => by simp only [take, length]
+| Nat.succ n, x :: xs, h =>
+  have ih : length (take n xs) = n :=
+    length_take_of_lt n xs (Nat.lt_of_succ_lt_succ h)
+  by simp only [take, length]
+     apply congrArg Nat.succ ih
+
+theorem List.reverse_singleton (x : α) : reverse [x] = [x] := rfl
+
+theorem List.map_map_append {α β γ δ : Type _} :
+  ∀ (xs : List α) (ys : List β) (f : γ → δ) (g : α → γ) (h : β → γ),
+  map f (map g xs ++ map h ys) = map (f ∘ g) xs ++ map (f ∘ h) ys
+| [], ys, f, g, h => map_map f h ys
+| x :: xs, ys, f, g, h => congrArg (f (g x) :: ·) (map_map_append xs ys f g h)
+
+theorem List.sum_map_const {xs : List α} {f} (k : Nat) :
+  (∀ x ∈ xs, f x = k) → (xs.map f).sum = k * xs.length := by
+  intro heq
+  induction xs with
+  | nil => rfl
+  | cons x xs ih =>
+    simp only [List.sum, List.length]
+    specialize ih (λ y hy => heq y (.tail _ hy))
+    rw [heq x (.head _), ih, Nat.mul_add, Nat.add_comm, Nat.mul_one]
+
+theorem List.length_bind {α β} {f : α → List β} {xs : List α} :
+    List.length (xs.bind f) = (xs.map (List.length ∘ f)).sum := by
+  induction xs with
+  | nil => rfl
+  | cons x xs ih =>
+    simp only [List.bind, List.map, List.join]
+    cases h : f x with
+    | nil =>
+      rw [List.nil_append, Function.comp, h, List.length_nil, List.sum,
+          Nat.zero_add]
+      exact ih
+    | cons y ys =>
+      rw [List.length_append, Function.comp, h, List.sum]
+      exact congrArg _ ih
+
+theorem List.sublist_self : ∀ (xs : List α), Sublist xs xs
+| [] => Sublist.slnil
+| x :: xs => Sublist.cons₂ x (sublist_self xs)
+
+theorem List.singleton_sublist_of_mem (y : α) :
+  ∀ (xs : List α), y ∈ xs → Sublist [y] xs
+| .(y) :: xs, List.Mem.head _ => Sublist.cons₂ y (nil_sublist xs)
+| x :: xs, List.Mem.tail .(x) h =>
+  Sublist.cons x (singleton_sublist_of_mem y xs h)
+
+theorem List.map_sublist_of_sublist :
+  (xs : List α) → (ys : List α) → (f : α → β) → Sublist xs ys →
+    Sublist (xs.map f) (ys.map f)
+| [], ys, f, h => nil_sublist (map f ys)
+| xs, x :: ys, f, Sublist.cons _ h =>
+  have ih := map_sublist_of_sublist xs ys f h
+  Sublist.cons (f x) ih
+| x :: xs, _ :: ys, f, Sublist.cons₂ _ h =>
+  have ih := map_sublist_of_sublist xs ys f h
+  Sublist.cons₂ (f x) ih
+
+theorem List.get_mem_cons_of_head_not_mem_getee {y :α} {xs ys : List α} {i} :
+  xs.get i ∈ y :: ys → y ∉ xs → xs.get i ∈ ys :=
+  λ hget hnmem =>
+  have hget_lem := get_mem xs i.val i.isLt
+  have hneq_lem := neq_of_mem_not_mem hget_lem hnmem
+  match mem_cons.mp hget with
+  | .inr htl => htl
+  | .inl heq => absurd heq hneq_lem
+
+theorem List.mem_append_singleton : ∀ (x : α) (xs : List α), x ∈ xs ++ [x]
+| x, [] => List.Mem.head _
+| x, y :: ys => List.Mem.tail _ (mem_append_singleton x ys)
+
+theorem List.mem_append_comm {v : α} {xs ys : List α} :
+  v ∈ xs ++ ys ↔ v ∈ ys ++ xs :=
+have flip : ∀ {as bs}, v ∈ as ++ bs → v ∈ bs ++ as :=
+  (λ h => h |> mem_append.mp |> Or.comm.mp |> mem_append.mpr)
+Iff.intro flip flip
+
+-- Slightly over-generalized "loop invariant" (we could make the preservation
+-- portion more specific, e.g., by providing `x ∈ xs` as an extra hypothesis)
+theorem List.foldr_invariant :
+  ∀ (p : β → Prop) (f : α → β → β) (z : β) (xs : List α),
+  p z → (∀ x a, p a → p (f x a)) → p (List.foldr f z xs)
+| _, _, _, [], h_init, _ => h_init
+| p, f, z, x :: xs, h_init, h_pres =>
+  h_pres x (foldr f z xs) (foldr_invariant p f z xs h_init h_pres)
