Table/BuiltinExtensions/List/Counts.lean
@@ -1,0 +1,144 @@
+import Table.BuiltinExtensions.List.Basic
+import Table.BuiltinExtensions.List.Filtering
+
+/-!
+`List.counts`, helper functions, and associated theorems.
+TODO: these proofs could probably be cleaned up a lot.
+-/
+
+def List.incrCounts {α} [DecidableEq α] :
+  List (α × Nat) → α → List (α × Nat)
+| [], v => [(v, 1)]
+| (t, n) :: rs, v =>
+  if t = v then (t, n + 1) :: rs else (t, n) :: incrCounts rs v
+
+def List.counts {α} [DecidableEq α] (xs : List α) : List (α × Nat) :=
+  xs.foldl (λ acc v => incrCounts acc v) []
+
+theorem List.map_fst_incrCounts_eq_map_fst [DecidableEq α] (x : α) :
+  ∀ (as : List (α × Nat)) (h : x ∈ map Prod.fst as),
+  map Prod.fst (incrCounts as x) = map Prod.fst as
+| (.(x), _) :: as, List.Mem.head _ => by simp only [map, incrCounts]
+| a :: as, List.Mem.tail _ h' =>
+  have ih := map_fst_incrCounts_eq_map_fst x as h'
+  match Decidable.em (a.1 = x) with
+  | .inl heq => by simp only [map, incrCounts, heq, ite_true, map]
+  | .inr hneq => by
+      simp only [hneq, ite_false, map, incrCounts]
+      exact congrArg _ ih
+
+theorem List.map_fst_incrCounts_eq_cons_fst [DecidableEq α] (x : α) :
+  ∀ (as : List (α × Nat)) (h : x ∉ map Prod.fst as),
+  map Prod.fst (incrCounts as x) = map Prod.fst as ++ [x] := by
+  intros as h
+  induction as with
+  | nil =>
+    simp only [incrCounts, map, HAppend.hAppend, Append.append, List.append]
+  | cons a as ih =>
+    simp only [map, incrCounts]
+    cases Decidable.em (a.1 = x) with
+    | inl heq =>
+      apply absurd h
+      apply not_not
+      simp only [map, heq]
+      apply List.Mem.head
+    | inr hneq =>
+      simp only [hneq, ite_false, map]
+      apply congrArg
+      apply ih
+      . intros hneg
+        apply h
+        apply List.Mem.tail _ hneg
+
+theorem List.length_uniqueAux_congr_append_cons_acc [DecidableEq α]
+  (x y : α) (as xs : List α) (cs : List α) :
+  length (uniqueAux xs (cs ++ x :: (as ++ [y]))) =
+  length (uniqueAux xs (cs ++ y :: x :: as)) := by
+  induction xs generalizing cs with
+  | nil =>
+    simp [uniqueAux]
+    rw [Nat.add_assoc,
+        Nat.add_comm (length cs),
+        ←Nat.add_assoc]
+  | cons z zs ih =>
+    have rearrange_mem :
+      (z ∈ cs ++ x :: (as ++ [y])) ↔ (z ∈ cs ++ y :: x :: as) := by
+      apply Iff.intro
+      . intros h
+        cases mem_append.mp h with
+        | inl hcs => exact mem_append_of_mem_left _ hcs
+        | inr hcons =>
+          apply mem_append_of_mem_right
+          rw [←cons_append] at hcons
+          cases mem_append.mp hcons with
+          | inl hxas => exact List.Mem.tail _ hxas
+          | inr hy =>
+            cases hy with
+            | tail _ _ => contradiction
+            | head _ => exact List.Mem.head _
+      . intros h
+        cases mem_append.mp h with
+        | inl hcs => exact mem_append_of_mem_left _ hcs
+        | inr hcons =>
+          apply mem_append_of_mem_right
+          cases hcons with
+          | head _ =>
+            apply List.Mem.tail
+            apply mem_append_of_mem_right
+            apply List.mem_singleton.mpr rfl
+          | tail _ hcons' =>
+            rw [←cons_append]
+            exact mem_append_of_mem_left _ hcons'
+
+    simp only [uniqueAux]
+    cases Decidable.em (z ∈ cs ++ x :: (as ++ [y])) with
+    | inl hin =>
+      simp only [hin, rearrange_mem.mp hin, ite_true]
+      apply ih
+    | inr hout =>
+      simp only [hout, rearrange_mem.not_iff_not_of_iff.mp hout, ite_false]
+      have rw_help (stuff) : (z :: (cs ++ stuff)) = ((z :: cs) ++ stuff) := rfl
+      rw [rw_help, rw_help]
+      apply ih
+
+theorem List.length_counts_aux [DecidableEq α]
+  (xs : List α) (acc : List (α × Nat)) :
+  List.length (foldl (λ acc v => incrCounts acc v) acc xs) =
+  List.length (uniqueAux xs (acc.map Prod.fst)) := by
+  induction xs generalizing acc with
+  | nil => simp [foldl, uniqueAux]
+  | cons x xs ih =>
+    simp only [uniqueAux, foldl]
+    cases acc with
+    | nil =>
+      simp only [incrCounts, map, List.not_mem_nil, ite_false]
+      apply ih
+    | cons a as =>
+      simp only [incrCounts]
+      cases Decidable.em (a.1 = x) with
+      | inl htrue =>
+        simp only [htrue, ite_true, incrCounts, map]
+        rw [if_pos]
+        . apply ih
+        . exact List.Mem.head _
+      | inr hfalse =>
+        simp only [hfalse, ite_false, incrCounts, map]
+        rw [ih]
+        cases Decidable.em (x ∈ map Prod.fst as) with
+        | inl hin =>
+          have : x ∈ a.1 :: map Prod.fst as := List.Mem.tail _ hin
+          simp only [this, ite_true, map, uniqueAux]
+          apply congrArg
+          apply congrArg
+          apply congrArg
+          exact map_fst_incrCounts_eq_map_fst x as hin
+        | inr hout =>
+          have : ¬ (x ∈ a.1 :: map Prod.fst as) := by
+            intros hneg; cases hneg; repeat contradiction
+          simp only [this, ite_false, map]
+          rw [map_fst_incrCounts_eq_cons_fst _ _ hout]
+          apply List.length_uniqueAux_congr_append_cons_acc _ _ _ _ []
+
+theorem List.length_counts [DecidableEq α] (xs : List α) :
+  xs.counts.length = xs.unique.length :=
+  length_counts_aux xs []
