Table/BuiltinExtensions/List/Filtering.lean
@@ -1,0 +1,369 @@
+import Table.BuiltinExtensions.Logic
+import Table.BuiltinExtensions.List.Basic
+import Table.BuiltinExtensions.List.Predicates
+
+/-!
+Contains theorems about `List.filter` as well as implementation of and theorems
+about filtering-like functions (`List.removeAllEq` and `List.unique` and its
+variants).
+-/
+
+def List.removeAllEq [DecidableEq α] (xs ys : List α) : List α :=
+  xs.filter (fun x => x ∉ ys)
+
+-- TODO: should we use `List.eraseDups` instead? (Uses BEq instead of DEq.)
+def List.uniqueAux {α} [DecidableEq α] : List α → List α → List α
+| [], acc => acc.reverse
+| x :: xs, acc => if x ∈ acc then uniqueAux xs acc else uniqueAux xs (x :: acc)
+
+def List.unique {α} [inst : DecidableEq α] (xs : List α) := uniqueAux xs []
+
+def List.unique' {α} [DecidableEq α] : List α → List α
+| [] => []
+| x :: xs =>
+  have : length (filter (fun x_1 => !decide (x_1 = x)) xs) < length xs + 1 :=
+    Nat.lt_succ_of_le (length_filter_le _ _)
+  x :: unique' (xs.filter (· ≠ x))
+termination_by xs => xs.length
+
+def List.filterSpec (p : α → Bool) : List α → List α
+| [] => []
+| x :: xs => if p x then x :: filterSpec p xs else filterSpec p xs
+
+theorem List.length_filterTR_le {α} (g : α → Bool) (xs : List α) :
+    ∀ rs : List α, List.length (List.filterTR.loop g xs rs)
+                   <= List.length xs + List.length rs :=
+by
+  induction xs with
+  | nil =>
+    intro rs
+    simp only [filter, filterTR.loop]
+    rw [List.length_reverse]
+    simp only [length, Nat.zero_add]
+    apply Nat.le.refl
+  | cons x xs ih =>
+    intro rs
+    simp only [filter, filterTR.loop]
+    cases (g x) with
+    | true => simp only
+              apply Nat.le_trans (ih (x::rs))
+              simp only [length]
+              rw [Nat.add_comm (length rs), Nat.add_assoc]
+              apply Nat.le.refl
+    | false => simp only [length]
+               apply Nat.le_trans (ih rs)
+               rw [Nat.add_comm (length xs) 1,
+                   Nat.add_assoc 1,
+                   Nat.add_comm 1,
+                   Nat.add_one]
+               apply Nat.le.step
+               apply Nat.le.refl
+
+
+theorem List.filter_eq_filterSpec : filter p xs = filterSpec p xs :=
+by induction xs with
+   | nil => simp [filter, filterSpec]
+   | cons x xs ih =>
+     simp only [filter, filterSpec]
+     cases p x with
+     | true => simp only [ite_true, ih]
+     | false => simp only [Bool.false_eq_true, ite_false, ih]
+
+theorem List.removeAll_singleton_hd_neq {α : Type _} [BEq α] :
+  ∀ (x : α) (y : α) (xs : List α),
+    ((x == y) = false) → removeAll (x :: xs) [y] = x :: removeAll xs [y] :=
+by intros x y xs hneq
+   simp only [removeAll, filter, elem, hneq, not]
+
+theorem List.removeAll_singleton_hd_eq [DecidableEq α] :
+  ∀ (x: α) (xs : List α), removeAll (x :: xs) [x] = removeAll xs [x] :=
+by intros x xs
+   simp [removeAll, filter, elem] -- previous filterAux too
+
+theorem List.removeAllEq_singleton_hd_eq [DecidableEq α] :
+  ∀ (x: α) (xs : List α), removeAllEq (x :: xs) [x] = removeAllEq xs [x] := by
+  intros x xs
+  simp [removeAllEq, filter, elem] -- previous filterAux too
+
+theorem List.removeAllEq_singleton_hd_neq {α : Type _} [DecidableEq α] :
+  ∀ (x : α) (y : α) (xs : List α),
+    x ≠ y → removeAllEq (x :: xs) [y] = x :: removeAllEq xs [y] :=
+by intro x y xs hneq
+   simp only [removeAllEq, filter, mem_singleton, hneq, not_false_eq_true,
+              decide_True, decide_not]
+
+theorem List.removeAllEq_singleton_nonelem_eq {α} [DecidableEq α] :
+  ∀ (xs : List α) (x : α), x ∉ xs → List.removeAllEq xs [x] = xs := by
+  intro xs x hnmem
+  induction xs with
+  | nil => rfl
+  | cons x' xs ih =>
+    rw [removeAllEq_singleton_hd_neq]
+    congr
+    apply ih
+    intro hneg
+    apply hnmem
+    apply Mem.tail
+    . exact hneg
+    . intro hneg'
+      rw [hneg'] at hnmem
+      apply hnmem
+      apply Mem.head
+
+-- BEGIN theorems originally used as helpers for `groupByKey`
+theorem List.uniqueAux_acc_append_filter {α} [DecidableEq α] :
+  ∀ (xs acc : List α),
+  uniqueAux xs acc = reverse acc ++ unique (xs.filter (· ∉ acc))
+| [], acc => by rw [filter, unique, uniqueAux, uniqueAux, reverse_nil,
+                    append_nil]
+| x :: xs, acc =>
+  have hterm : length (filter (λ a => !decide (a ∈ acc)) xs)
+                < Nat.succ (length xs) :=
+    Nat.lt_of_le_of_lt (m := length xs) (length_filter_le _ _) (Nat.lt.base _)
+  have hterm' : length xs < (length xs).succ := Nat.le.refl
+  have ih₁ := uniqueAux_acc_append_filter xs acc
+  have ih₂ := uniqueAux_acc_append_filter xs (x :: acc)
+  have ih₃ :=
+    uniqueAux_acc_append_filter (filter (λ a => decide ¬a ∈ acc) xs) [x]
+  by
+    simp only [uniqueAux, filter]  -- previously filterAux
+    cases Decidable.em (x ∈ acc) with
+    | inl hin =>
+      simp only [hin, ite_true, not_true_eq_false, decide_False]
+      rw [ih₁]
+    | inr hout =>
+      -- Case x is not already in the accumulator
+      simp only [hout, ite_false, not_false_eq_true, decide_True]
+      -- next line previously filterAux
+      simp only [reverse_singleton, singleton_append, unique,
+                 uniqueAux, List.not_mem_nil, ite_false]
+      rw [ih₂]
+      simp only [reverse_cons, append_assoc, singleton_append]
+      apply congrArg
+      simp only [unique]
+      rw [ih₃]
+      simp [unique]
+termination_by xs ac => xs.length
+
+theorem List.uniqueAux_acc_append {α} [DecidableEq α] (xs : List α)
+  (acc : List α) (h : ∀ x, x ∈ xs → ¬ (x ∈ acc)) :
+  uniqueAux xs acc = reverse acc ++ unique xs := by
+  have : filter (fun a => decide ¬a ∈ acc) xs = xs := by
+    induction xs with
+    | nil => simp [filter]
+    | cons x xs ih =>
+      simp only [filter]
+      have : decide (¬x ∈ acc) = true := by simp [h x (Mem.head _)]
+      rw [this]
+      simp only
+      rw [ih]
+      . intros x hx
+        apply h x (Mem.tail _ hx)
+  rw [uniqueAux_acc_append_filter]
+  cases xs with
+  | nil => apply congrArg; simp [filter]
+  | cons x xs =>
+    apply congrArg
+    rw [this]
+
+theorem List.length_uniqueAux {α} [DecidableEq α]
+  (xs : List α) (acc : List α) (h : ∀ x, x ∈ xs → ¬ (x ∈ acc)) :
+  length (uniqueAux xs acc) = length (unique xs) + length acc := by
+  rw [uniqueAux_acc_append _ _ h, length_append, length_reverse, Nat.add_comm]
+
+def List.memT_filter_false_of_memT {α} {x : α} {p : α → Bool} :
+  ∀ {xs : List α}, MemT x xs → p x = true → MemT x (filter p xs)
+| _, .hd _ _, heq => by
+  simp only [filter, heq]
+  apply MemT.hd
+| x' :: xs, .tl _ htl, heq =>
+  if h : p x'
+  then by
+    simp only [filter, h]
+    apply MemT.tl
+    apply memT_filter_false_of_memT htl heq
+  else by
+    simp only [filter, h]
+    apply memT_filter_false_of_memT htl heq
+
+-- TODO: if we want `pivotWider` to run in a reasonable amount of time, probably
+-- want to write this as a proof term
+def List.memT_unique_of_memT {α} [DecidableEq α]
+  : ∀ {x : α} {xs : List α}, MemT x xs → MemT x xs.unique
+| x, .(x) :: xs, .hd _ _ => by
+  unfold unique
+  unfold uniqueAux
+  simp only [not_mem_nil, ite_false]
+  rw [uniqueAux_acc_append_filter]
+  apply MemT.hd _ _
+| x, y :: xs, .tl .(y) htl =>
+  -- TODO: we keep using this...probably make it a separate simp lemma
+  have hterm : length (filter (λ a => !decide (a = y)) xs) < length xs + 1 :=
+    Nat.lt_of_le_of_lt (m := length xs) (length_filter_le _ _) (Nat.lt.base _)
+  by
+  simp only [unique, uniqueAux, not_mem_nil, ite_false]
+  simp only [uniqueAux_acc_append_filter]
+  simp only [reverse_singleton, singleton_append]
+  apply Decidable.byCases (p := x = y)
+  . intro heq
+    rw [←heq]
+    apply MemT.hd
+  . intro hneq
+    apply MemT.tl
+    apply memT_unique_of_memT
+    apply memT_filter_false_of_memT
+    exact htl
+    have hnin : ¬ x ∈ [y] := by
+      intro hneg
+      cases hneg <;>
+      contradiction
+    simp only [hnin, not_false_eq_true, decide_True]
+termination_by x xs hmem => xs.length
+-- END `groupByKey
+
+-- BEGIN `leftJoin` spec 4 helpers
+theorem List.mem_filter_of_mem_filter_imp {p q : α → Bool} {y : α}
+  {xs : List α} :
+  (∀ x, p x → q x) → y ∈ xs.filter p → y ∈ xs.filter q := by
+  intro hpq hp
+  induction xs with
+  | nil => contradiction
+  | cons x xs ih =>
+    cases Decidable.em (p x) with
+    | inl htrue =>
+      have hq := hpq x htrue
+      simp only [htrue, List.filter_cons_of_pos, List.mem_cons, hq] at hp ⊢
+      cases hp with
+      | inl heq => exact .inl heq
+      | inr htl => exact .inr (ih htl)
+    | inr hfalse =>
+      simp only [List.filter, hfalse] at hp
+      cases Decidable.em (q x) with
+      | inl hqtrue =>
+        simp only [List.filter, hqtrue]
+        apply List.Mem.tail
+        apply ih hp
+      | inr hqfalse =>
+        simp only [List.filter, hqfalse]
+        exact ih hp
+
+theorem List.not_mem_filter_neq [DecidableEq α] (y : α) : ∀ (xs : List α),
+  y ∉ filter (· ≠ y) xs
+  | x :: xs, h => by
+    simp only [filter] at h
+    cases hdec : decide (x = y) with
+    | true =>
+      simp only [ne_eq, decide_not, hdec, Bool.not_true] at h
+      simp only [←decide_not, ←ne_eq] at h
+      exact not_mem_filter_neq _ _ h
+    | false =>
+      simp only [ne_eq, decide_not, hdec, Bool.not_false, mem_cons] at h
+      cases h with
+      | inl heq => cases heq; simp only [decide_True, Bool.true_eq_false] at hdec
+      | inr hmem =>
+        simp only [←decide_not, ←ne_eq] at hmem
+        exact not_mem_filter_neq _ _ hmem
+
+theorem List.filter_mem_pred_true :
+  ∀ (xs : List α) (pred : α → Bool), ∀ r ∈ xs.filter pred, pred r = true
+  | [], pred => λ r hr => nomatch hr
+  | x :: xs, pred =>
+    if h : pred x
+    then by
+      intro r hr
+      simp only [filter, h] at hr
+      cases hr with
+      | head => exact h
+      | tail _ htl =>
+        apply filter_mem_pred_true _ _ _ htl
+    else λ r hr => by
+      simp only [filter, h] at hr
+      apply filter_mem_pred_true _ _ _ hr
+
+
+theorem List.unique_sublist {xs ys : List α} :
+    Unique ys → xs <+ ys → Unique xs := by
+  intro hunique hsubl
+  induction hsubl with
+  | slnil => exact .nil
+  | cons x hsubl' ih =>
+    apply ih
+    cases hunique
+    repeat assumption
+  | cons₂ x hsubl' ih =>
+    constructor
+    . cases hunique
+      intro hneg
+      have := Sublist.mem hneg hsubl'
+      contradiction
+    . apply ih
+      cases hunique
+      repeat assumption
+
+unseal List.unique' in
+theorem List.unique_eq_unique' [DecidableEq α] : ∀ (xs : List α),
+  unique xs = unique' xs
+  | [] => rfl
+  | x :: xs =>
+  by
+    simp only [unique, unique', uniqueAux, not_mem_nil, ite_false]
+    rw [uniqueAux_acc_append_filter, reverse_singleton, singleton_append]
+    apply congrArg
+    simp only [mem_cons, not_mem_nil, or_false, decide_not, ne_eq]
+    have : length (filter (fun x_1 => !decide (x_1 = x)) xs) < 1 + length xs :=
+    by
+      apply Nat.lt_of_le_of_lt
+      apply length_filter_le
+      rw [Nat.add_comm]
+      apply Nat.lt.base
+    apply unique_eq_unique'
+termination_by xs => xs.length
+
+unseal List.unique' in
+theorem List.unique'_sublist [DecidableEq α] : ∀ (xs : List α),
+  List.unique' xs <+ xs
+  | [] => .slnil
+  | x :: xs =>
+    have : (filter (fun x_1 => !decide (x_1 = x)) xs).length < xs.length + 1 :=
+      Nat.lt_succ_of_le (length_filter_le _ _)
+    Sublist.cons₂ _ $
+      Sublist.trans (List.unique'_sublist _) (List.filter_sublist _)
+termination_by xs => xs.length
+
+unseal List.unique' in
+theorem List.unique'_Unique [DecidableEq α] : ∀ (xs : List α),
+  Unique xs.unique'
+  | [] => .nil
+  | x :: xs =>
+    have : (filter (fun x_1 => !decide (x_1 = x)) xs).length < xs.length + 1 :=
+      Nat.lt_succ_of_le (length_filter_le _ _)
+    .cons (mt (Sublist.mem.swap (unique'_sublist _)) (not_mem_filter_neq x xs))
+          (unique'_Unique _)
+termination_by xs => xs.length
+-- END `leftJoin` spec 4 helpers
+
+theorem List.length_uniqueAux_le [DecidableEq α] (xs : List α) :
+  ∀ as, length (uniqueAux xs as) ≤ length xs + length as := by
+  induction xs with
+  | nil => simp [uniqueAux]
+  | cons x xs ih =>
+    intros as
+    cases Decidable.em (x ∈ as) with
+    | inl h =>
+      simp only [length, uniqueAux, h, ite_true]
+      apply Nat.le_trans
+      apply ih
+      rw [Nat.add_assoc, Nat.add_comm 1, ←Nat.add_assoc]
+      apply Nat.le_step
+      simp
+    | inr h =>
+      simp only [length, uniqueAux, h, ite_false]
+      apply Nat.le_trans
+      apply ih
+      simp only [length]
+      rw [Nat.add_comm _ 1, Nat.add_assoc]
+      apply Nat.le_refl
+
+theorem List.length_unique_le [DecidableEq α] (xs : List α) :
+  length (unique xs) ≤ length xs :=
+List.length_uniqueAux_le xs []
