Table/BuiltinExtensions/List/GroupByKey.lean
@@ -1,0 +1,527 @@
+import Table.BuiltinExtensions.Logic
+import Table.BuiltinExtensions.List.Filtering
+import Table.BuiltinExtensions.List.Predicates
+
+/-!
+Implementation of and lemmas about `groupByKey`, used in the `groupBy` function.
+Contains infrastructure for `groupBy`, as well as some extra proofs that
+aren't used but might be useful in the future.
+-/
+
+/-
+Takes a list `kvs` consisting of (key, value) pairs and a key `k` and returns
+a tuple `(vs, kvs')` where `vs` are all values having key `k` and `kvs'` is the
+sublist of `kvs` with key entries not equal to `k`.
+-/
+def List.matchKey {κ ν} [DecidableEq κ]
+    : List (κ × ν) → κ → List ν × List (κ × ν)
+| [], _ => ([], [])
+| (k, v) :: kvs, x =>
+  let res := matchKey kvs x
+  if k = x
+  then (v :: res.1, res.2)
+  else (res.1, (k, v) :: res.2)
+
+theorem List.matchKey_snd_length {κ ν} [DecidableEq κ] :
+    ∀ (xs : List (κ × ν)) (k : κ), (matchKey xs k).2.length ≤ xs.length :=
+by intros xs k
+   induction xs with
+   | nil => exact Nat.le.refl
+   | cons x xs ih =>
+     simp only [matchKey]
+     apply @Decidable.byCases (x.1=k) _
+     . intros heq
+       simp only [heq]
+       rw [ite_true]
+       simp only [Prod.snd]
+       apply Nat.le_step
+       exact ih
+     . intros hneq
+       simp only [hneq]
+       rw [ite_false]
+       simp only [Prod.fst]
+       apply Nat.succ_le_succ
+       exact ih
+
+theorem List.matchKey_lengths_sum {κ ν} [inst : DecidableEq κ] :
+  ∀ (xs : List (κ × ν)) (k : κ),
+  (matchKey xs k).1.length + (matchKey xs k).2.length = xs.length :=
+by intros xs k
+   induction xs with
+   | nil => rfl
+   | cons x xs ih =>
+     simp only [matchKey]
+     cases inst x.1 k with
+     | isFalse hfalse =>
+       simp only [hfalse, ite_false, List.length]
+       rw [←Nat.add_assoc]
+       apply congrArg (·+1) ih
+     | isTrue htrue =>
+       simp only [htrue, ite_true, List.length]
+       rw [Nat.add_assoc, Nat.add_comm 1, ←Nat.add_assoc]
+       apply congrArg (·+1) ih
+
+theorem List.not_mem_matchKey_self_map_snd {κ ν} [DecidableEq κ]
+  (k : κ) (kvs : List (κ × ν)) :
+  k ∉ map Prod.fst (matchKey kvs k).snd := by
+  intro hneg
+  induction kvs with
+  | nil => cases hneg
+  | cons kv kvs ih =>
+    apply ih
+    simp only [matchKey] at hneg
+    cases Decidable.em (kv.fst = k) with
+    | inl heq =>
+      simp only [heq, ite_true] at hneg
+      assumption
+    | inr hneq =>
+      simp only [hneq, ite_false] at hneg
+      simp only [map] at hneg
+      cases hneg with
+      | head => exact absurd rfl hneq
+      | tail _ h => exact h
+
+theorem List.fst_mem_of_pair_mem : ∀ (x : α) (y : β) (ps : List (α × β)),
+  (x, y) ∈ ps → x ∈ (map Prod.fst ps)
+| x, y, [], hxy => by contradiction
+| x, y, _ :: ps, List.Mem.head _ => List.Mem.head _
+| x, y, _ :: ps, List.Mem.tail a h => Mem.tail _ $ fst_mem_of_pair_mem x y ps h
+
+theorem List.matchKey_snd_keys_neq_k [DecidableEq κ] (xs : List (κ × ν)) :
+  ∀ e, e ∈ (matchKey xs k).snd → e.fst ≠ k := λ e he hneg =>
+  absurd (List.fst_mem_of_pair_mem e.1 e.2 (matchKey xs k).snd he)
+         (hneg ▸ not_mem_matchKey_self_map_snd k xs)
+
+def List.uniqueFoldl [DecidableEq α] (xs : List α) :=
+  xs.foldl (λ acc x => if x ∈ acc then acc else acc ++ [x]) []
+
+-- theorem List.unique_eq_uniqueFold_aux [DecidableEq α] :
+--   ∀ (xs : List α) (acc : List α),
+--   uniqueAux xs acc =
+--     foldl (λ acc x => if x ∈ acc then acc else acc ++ [x]) (reverse acc) xs := sorry
+  --   by
+  -- intros xs acc
+  -- induction xs generalizing acc with
+  -- | nil => simp [uniqueAux, foldl]
+  -- | cons x xs ih =>
+  --   simp only [uniqueAux, foldl]
+  --   cases Decidable.em (x ∈ acc) with
+  --   | inl h =>
+  --     simp only [h, ite_true]
+  --     conv =>
+  --       rhs
+  --       lhs
+  --       have : (if x ∈ reverse acc then reverse acc else reverse acc ++ [x]) =
+  --              if x ∈ acc then reverse acc else reverse acc ++ [x] := by rw [← mem_reverse]
+
+
+-- theorem List.unique_eq_uniqueFold [DecidableEq α] :
+--   ∀ (xs : List α), unique xs = uniqueFoldl xs := by
+--   intros xs
+--   induction xs with
+--   | nil => simp [unique, uniqueFoldl, uniqueAux, foldl]
+--   | cons x xs ih =>
+--     simp only [unique, uniqueFoldl, uniqueAux]
+--     simp only [List.not_mem_nil, ite_false]
+--     rw [unique_eq_uniqueFold_aux]
+--     simp only [foldl]
+--     apply congrArg
+--     rfl
+
+theorem List.all_pred {p : α → Prop} [DecidablePred p] {xs : List α} :
+  xs.all (λ x => decide (p x)) ↔ ∀ x, x ∈ xs → p x :=
+  ⟨λ h x hx => of_decide_eq_true (List.all_eq_true.mp h x hx),
+   λ h => List.all_eq_true.mpr (λ x hx => decide_eq_true (h x hx))⟩
+
+theorem List.length_sublist_le {α} {xs ys : List α} :
+  xs <+ ys → xs.length ≤ ys.length
+  | .slnil => .refl
+  | .cons _ hsubl => Nat.le_succ_of_le (length_sublist_le hsubl)
+  | .cons₂ _ hsubl => Nat.succ_le_succ (length_sublist_le hsubl)
+
+theorem List.matchKey_fst_eq_filter_k_map_snd {κ ν} [inst : DecidableEq κ] :
+  ∀ (xs : List (κ × ν)) (k : κ),
+    (matchKey xs k).1 = (xs.filter (λ x => x.1 = k)).map Prod.snd :=
+by intros xs k
+   induction xs with
+   | nil => rfl
+   | cons x xs ih =>
+     simp only [matchKey]
+     cases inst x.1 k with
+     | isFalse hfalse =>
+       simp only [hfalse, ite_false, ih, filter]
+       exact rfl
+     | isTrue htrue =>
+       simp [htrue, ite_true, filter, ih, map]
+
+theorem List.matchKey_length_lt {κ} [DecidableEq κ] {ν}
+                                (k : κ) (kvs : List (κ × ν)) :
+  (matchKey kvs k).2.length < kvs.length.succ :=
+  Nat.lt_of_succ_le $ Nat.succ_le_succ $ matchKey_snd_length kvs k
+
+def List.groupByKey {κ} [DecidableEq κ] {ν} : List (κ × ν) → List (κ × List ν)
+| [] => []
+| (k, v) :: kvs =>
+  have h_help : (matchKey kvs k).2.length < kvs.length.succ :=
+    matchKey_length_lt k kvs
+
+  let fms := matchKey kvs k
+  (k, v :: fms.1) :: groupByKey fms.2
+termination_by xs => xs.length
+decreasing_by assumption
+
+theorem List.groupByKey_matchKey_snd_length_cons [DecidableEq κ]
+  (k : κ) (v : ν) (xs : List (κ × ν)) :
+  1 + length (groupByKey (matchKey ((k, v) :: xs) k).snd)
+    = (groupByKey ((k, v) :: xs)).length :=
+calc
+  1 + length (groupByKey (matchKey ((k, v) :: xs) k).2)
+  = 1 + length (groupByKey (matchKey xs k).2) :=
+    by simp only [matchKey, length, ite_true]
+  _ = length (groupByKey (matchKey xs k).2) + 1 := Nat.add_comm _ _
+  _ = length ((k, v :: (matchKey xs k).1) :: groupByKey (matchKey xs k).2) :=
+    rfl
+  _ = length (groupByKey ((k, v) :: xs)) := by simp only [matchKey, groupByKey]
+
+theorem List.length_uniqueAux_matchKey {κ ν} [DecidableEq κ]
+  (xs : List (κ × ν)) (k : κ) :
+  ∀ (acc : List κ) (hk : k ∈ acc),
+  (uniqueAux (map Prod.fst xs) acc).length
+  = (uniqueAux (map Prod.fst (matchKey xs k).snd) acc).length :=
+by induction xs with
+   | nil => intros; simp [uniqueAux]
+   | cons x xs ih =>
+     intros acc hk
+     simp only [length, uniqueAux]
+     cases Decidable.em (x.fst ∈ acc) with
+     | inl hin =>
+       simp only [hin, ite_true, matchKey]
+       rw [ih _ hk]
+       cases Decidable.em (x.1 = k) with
+       | inl heq => simp only [heq, ite_true]
+       | inr hneq => simp only [hneq, ite_false, map, uniqueAux, hin, ite_true]
+     | inr hout =>
+       simp only [hout, ite_false, matchKey]
+       cases Decidable.em (x.1 = k) with
+       | inl heq =>
+         apply absurd hk
+         rw [heq] at hout
+         exact hout
+       | inr hneq =>
+         rw [ih _ (List.Mem.tail _ hk)]
+         simp only [hneq, ite_false, uniqueAux, hout]
+
+instance (y : Nat) : Decidable (∀ x : Nat, x - y = x) :=
+  if h : y = 0
+  then Decidable.isTrue (λ x => by rw [h]; simp)
+  else Decidable.isFalse (λ x => by
+    have h1 : 1 - y = 1 := x 1
+    have : y > 0 := Nat.zero_lt_of_ne_zero h
+    have := Nat.sub_lt (Nat.lt.base 0) this
+    apply absurd h1
+    apply Nat.ne_of_lt this)
+
+theorem List.length_groupByKey {κ} [DecidableEq κ] {ν} :
+  ∀ (xs : List (κ × ν)),
+  length (groupByKey xs) = (xs.map Prod.fst).unique.length
+| [] => by simp only [groupByKey, unique, uniqueAux, length]
+| (k, v) :: xs => by
+  have hterm : length (matchKey xs k).snd < Nat.succ (length xs) :=
+    Nat.lt_of_succ_le $ Nat.succ_le_succ $ matchKey_snd_length xs k
+  have ih := length_groupByKey (matchKey xs k).2
+  simp only [map, unique, uniqueAux, List.not_mem_nil, ite_false, groupByKey]
+  -- This needs to be a separate `simp` to ensure proper ordering
+  simp only [length]
+  rw [length_uniqueAux_matchKey _ k _ $ List.Mem.head _]
+  rw [ih]
+  apply Eq.symm
+  apply List.length_uniqueAux (acc := [k])
+  intro x
+  rw [mem_singleton]
+  intro hmem hneg
+  have := not_mem_matchKey_self_map_snd x xs
+  rw [←hneg] at hmem
+  exact this hmem
+termination_by xs => length xs
+decreasing_by assumption
+-- END `groupByKey` - `groupBy` spec 4
+
+-- BEGIN `groupByRetentive` spec 4 (this might simplify some stuff above?)
+
+theorem List.matchKey_snd_sublist [DecidableEq κ] :
+  ∀ (k : κ) (kvs : List (κ × ν)), (matchKey kvs k).snd <+ kvs
+| _, [] => Sublist.slnil
+| k, (kv :: kvs) =>
+  have ih := matchKey_snd_sublist k kvs
+  if h : kv.fst = k
+  then by simp only [matchKey, h, ite_true]; exact Sublist.cons _ ih
+  else by simp only [matchKey, h, ite_true]; exact Sublist.cons₂ _ ih
+
+theorem List.matchKey_snd_sublist_of_sublist [DecidableEq κ] :
+  ∀ (k : κ) (xs ys : List (κ × ν)),
+  xs <+ ys → (matchKey xs k).snd <+ (matchKey ys k).snd := by
+  intro k xs ys h
+  induction h with
+  | slnil => constructor
+  | cons x' h' ih =>
+    simp only [matchKey]
+    cases Decidable.em (x'.fst = k) with
+    | inl heq => simp only [heq, ite_true]; apply ih
+    | inr hneq => simp only [hneq, ite_false]; apply Sublist.cons _ ih
+  | cons₂ x' h' ih =>
+    simp only [matchKey]
+    cases Decidable.em (x'.fst = k) with
+    | inl heq => simp only [heq, ite_true]; assumption
+    | inr hneq =>
+      simp only [hneq, ite_false]
+      apply Sublist.cons₂ _ ih
+
+theorem List.fst_groupByKey_sublist [DecidableEq κ] : ∀ (kvs : List (κ × ν)),
+  map Prod.fst (groupByKey kvs) <+ map Prod.fst kvs
+| [] => groupByKey.eq_1 (κ := κ) ▸ Sublist.slnil
+| (k, v) :: kvs =>
+  have hterm := matchKey_length_lt k kvs
+  have ih := fst_groupByKey_sublist (matchKey kvs k).snd
+  have hsubl := matchKey_snd_sublist k kvs
+  by
+    simp only [groupByKey]
+    exact Sublist.cons₂ _ $
+    Sublist.trans ih (map_sublist_of_sublist _ _ _ hsubl)
+termination_by kvs => kvs.length
+
+-- It would be nice to do this fully in tactic mode, but there doesn't seem to
+-- be a way to retain unused `have`s as termination hints in tactic mode
+theorem List.mem_fst_matchKey_key_or_snd [DecidableEq κ] :
+  ∀ {ys : List (κ × ν)} {x : κ},
+  x ∈ map Prod.fst ys → ∀ k, x = k ∨ x ∈ map Prod.fst (matchKey ys k).snd :=
+λ {ys x} hx k =>
+  if h : x = k
+  then Or.inl h
+  else Or.inr $
+    match ys with
+    | (k', v) :: ys =>
+      have h_term : length (matchKey ys k).snd < Nat.succ (length ys) :=
+        matchKey_length_lt k ys
+      have h_term' : length ys < Nat.succ (length ys) := Nat.le.refl
+      by
+      simp only [matchKey]
+      cases Decidable.em (k' = k) with
+      | inl hkeq =>
+        simp only [hkeq, ite_true]
+        have : x ∈ map Prod.fst ys := by
+          cases hx with
+          | head => contradiction
+          | tail => assumption
+        have ih := mem_fst_matchKey_key_or_snd this k
+        cases ih with
+        | inl => contradiction
+        | inr hmem => exact hmem
+      | inr hkneq =>
+        simp only [hkneq, ite_false]
+        simp only [map]
+        cases Decidable.em (x = k') with
+        | inl hxeq => rw [hxeq]; apply Mem.head
+        | inr hxneq =>
+          apply Mem.tail
+          have : x ∈ map Prod.fst (matchKey ys k).snd := by
+            cases hx with
+            | head => contradiction
+            | tail _ htail =>
+              have := mem_fst_matchKey_key_or_snd htail k
+              cases this with
+              | inl => contradiction
+              | inr => assumption
+          have ih := mem_fst_matchKey_key_or_snd this k'
+          cases ih with
+          | inl => contradiction
+          | inr => assumption
+termination_by ys x hx k => ys.length
+
+-- TODO: avoid copy/paste?
+theorem List.mem_fst_groupByKey_key_or_snd [DecidableEq κ] :
+  ∀ {ys : List (κ × ν)} {x : κ},
+  x ∈ map Prod.fst ys →
+    ∀ k, x = k ∨ x ∈ map Prod.fst (groupByKey (matchKey ys k).snd) :=
+λ {ys x} hx k =>
+  if h : x = k
+  then Or.inl h
+  else Or.inr $
+    match ys with
+    | (k', v) :: ys =>
+      have h_term : length (matchKey ys k).snd < Nat.succ (length ys) :=
+        matchKey_length_lt k ys
+      have h_term' : length ys < Nat.succ (length ys) := Nat.le.refl
+      by
+      simp only [matchKey]
+      cases Decidable.em (k' = k) with
+      | inl hkeq =>
+        simp only [hkeq, ite_true]
+        have : x ∈ map Prod.fst ys := by
+          cases hx with
+          | head => contradiction
+          | tail => assumption
+        have ih := mem_fst_groupByKey_key_or_snd this k
+        cases ih with
+        | inl => contradiction
+        | inr hmem => exact hmem
+      | inr hkneq =>
+        simp only [hkneq, ite_false]
+        simp only [groupByKey]
+        simp only [map]
+        cases Decidable.em (x = k') with
+        | inl hxeq => rw [hxeq]; apply Mem.head
+        | inr hxneq =>
+          apply Mem.tail
+          have : x ∈ map Prod.fst (matchKey ys k).snd := by
+            cases hx with
+            | head => contradiction
+            | tail _ htail =>
+              have := mem_fst_matchKey_key_or_snd htail k
+              cases this with
+              | inl => contradiction
+              | inr => assumption
+          have ih := mem_fst_groupByKey_key_or_snd this k'
+          cases ih with
+          | inl => contradiction
+          | inr => assumption
+termination_by ys x hx k => ys.length
+
+/-
+Although tempting, the stronger claim
+  `xs <+ ys → map Prod.fst (groupByKey xs) <+ map Prod.fst (groupByKey ys)`
+does not hold, as the following counterexample illustrates:
+
+* `List.groupByKey [("a", 1), ("b", 2), ("a", 3)]`
+* `List.groupByKey [("b", 2), ("a", 3)]`
+
+Also, the initial hypothesis is a bit stricter than it needs to be:
+`(∀ x, x ∈ xs → x ∈ ys)` would suffice.
+-/
+unseal List.groupByKey in
+theorem List.all_in_map_fst_groupByKey_of_sublist [DecidableEq κ] :
+  ∀ {xs ys : List (κ × ν)},
+  xs <+ ys →
+    ∀ x, x ∈ map Prod.fst (groupByKey xs) → x ∈ map Prod.fst (groupByKey ys)
+| _, _, @Sublist.cons _ xs ys (k, v) hsubl, x, hx =>
+  if heq : x = k
+  then heq ▸ Mem.head _
+  else
+    have hterm : ys.length < Nat.succ ys.length := Nat.le.refl
+    have ih := all_in_map_fst_groupByKey_of_sublist hsubl x hx
+    have hor : x = k ∨ x ∈ map Prod.fst (groupByKey (matchKey ys k).snd) :=
+      mem_fst_groupByKey_key_or_snd
+        (Sublist.mem ih (fst_groupByKey_sublist ys)) k
+    Mem.tail k $
+    match hor with
+    | .inl hxeq => absurd hxeq heq
+    | .inr hmem => hmem
+| _, _, @Sublist.cons₂ _ xs ys (k, v) hsubl, x, hx => by
+    simp only [groupByKey]
+    simp only [map]
+    simp only [groupByKey] at hx
+    simp only [map] at hx
+    cases hx with
+    | head => constructor
+    | tail _ htail =>
+      apply Mem.tail
+      have : (matchKey xs k).snd <+ (matchKey ys k).snd :=
+        matchKey_snd_sublist_of_sublist _ _ _ hsubl
+      have hterm := matchKey_length_lt k ys
+      apply all_in_map_fst_groupByKey_of_sublist this
+      assumption
+termination_by xs ys hsubl x hx => ys.length
+
+-- #check @List.not_mem_matchKey_self_snd
+-- #check @List.matchKey_snd_sublist
+-- #check @List.matchKey_snd_sublist_of_sublist
+-- theorem List.map_groupByKey_matchKey_wip [DecidableEq κ] {k : κ} {kvs : List (κ × ν)} :
+--   ∀ x, x ∈ map Prod.fst (groupByKey (matchKey kvs k).snd) → x ∈ map Prod.fst (groupByKey kvs) := by
+--   intro x hx
+--   induction kvs with
+--   | nil => simp only [groupByKey, map] at hx; contradiction
+--   | cons kv kvs ih =>
+--     cases kv with | mk k' v =>
+--     -- simp only [matchKey] at hx
+--     simp only [groupByKey]
+--     simp only [map]
+--     cases Decidable.em (x = k') with
+--     | inl heq =>
+--       rw [heq]
+--       apply Mem.head
+--     | inr hneq =>
+--       simp only [matchKey] at hx
+--       apply Mem.tail
+--       cases Decidable.em (k' = k) with
+--       | inl heq' =>
+--         simp only [heq', ite_true] at hx
+--         rw [heq']
+--         apply hx
+--       | inr hneq' =>
+--         simp only [hneq', ite_false] at hx
+--         simp only [groupByKey] at hx
+--         simp only [map] at hx
+--         have := matchKey_snd_sublist k' (matchKey kvs k).snd
+--         sorry
+
+-- The converse is also true, but we don't need it here
+unseal List.groupByKey in
+theorem List.mem_fsts_of_mem_fsts_groupByKey [DecidableEq κ] (kvs : List (κ × ν)) :
+  k ∈ map Prod.fst (groupByKey kvs) → k ∈ map Prod.fst kvs := by
+  intro h
+  induction kvs with
+  | nil => contradiction
+  | cons kv kvs ih =>
+    cases kv with | mk k₀ v₀ =>
+    simp only [groupByKey] at h
+    simp only [map] at h
+    simp only [map]
+    cases h with
+    | head => apply Mem.head
+    | tail _ htail =>
+      apply Mem.tail
+      apply ih
+      apply all_in_map_fst_groupByKey_of_sublist (matchKey_snd_sublist k₀ kvs)
+      assumption
+
+-- Instead of being separate, this could just be folded into
+-- `groupByKey_fsts_no_duplicates`
+theorem List.key_not_mem_fst_groupByKey_matchKey_snd [DecidableEq κ]
+  (kvs : List (κ × ν)) (k : κ) :
+  k ∉ map Prod.fst (groupByKey (matchKey kvs k).snd) :=
+  mt (List.mem_fsts_of_mem_fsts_groupByKey (matchKey kvs k).snd)
+    (List.not_mem_matchKey_self_map_snd _ _)
+
+-- TODO: almost certainly need something more general for the induction
+unseal List.groupByKey in
+theorem List.groupByKey_fsts_no_duplicates [DecidableEq κ] :
+  ∀ (kvs : List (κ × ν)), Unique $ (groupByKey kvs).map Prod.fst
+| [] => Unique.nil
+| (k, v) :: kvs =>
+  have h_help : (matchKey kvs k).2.length < kvs.length.succ :=
+    matchKey_length_lt k kvs
+  Unique.cons
+    (List.key_not_mem_fst_groupByKey_matchKey_snd _ _)
+    (groupByKey_fsts_no_duplicates (matchKey kvs k).2)
+termination_by xs => xs.length
+decreasing_by assumption
+
+theorem List.mem_of_mem_injective_map (f : α → β) (hf : Injective f) :
+  ∀ (x : α) (xs : List α),
+  f x ∈ map f xs ↔ x ∈ xs :=
+λ _ xs => Iff.intro
+  (λ h =>
+    have ⟨_, hb⟩ := mem_map.mp h
+    have hbeqx := hf _ _ hb.right
+    Eq.subst (motive := λ a => a ∈ xs) hbeqx hb.left
+  )
+  (mem_map_of_mem _)
+
+theorem List.unique_of_map_injective_unique
+  (f : α → β) (hf : Injective f) : ∀ (xs : List α) (hxs : Unique xs),
+  Unique $ map f xs
+| [], hxs => Unique.nil
+| x :: xs, Unique.cons hxnin hndxs =>
+  Unique.cons
+    (λ hneg => absurd ((mem_of_mem_injective_map f hf x xs).mp hneg) hxnin)
+    (unique_of_map_injective_unique f hf xs hndxs)
+-- END `groupByRetentive` spec 4
