Table/BuiltinExtensions/List/MergeSort.lean
@@ -1,0 +1,194 @@
+/-!
+Merge sort for lists. This implementation was written before merge-sort was
+added to the library; we continue to use it because of proof dependencies.
+-/
+
+def List.split {α} : List α → List α × List α
+| [] => ([], [])
+| [x] => ([x], [])
+| x₁ :: x₂ :: xs =>
+  let (ys, zs) := split xs;
+  (x₁ :: ys, x₂ :: zs)
+
+theorem List.split_length_fst' {α} :
+    ∀ (xs : List α), (split xs).fst.length ≤ xs.length
+| [] => Nat.le.refl
+| [x] => Nat.le.refl
+| x₁ :: x₂ :: xs =>
+  have ih := split_length_fst' xs;
+  by simp only [split, length]
+     apply Nat.le.step
+     apply Nat.succ_le_succ
+     apply ih
+
+theorem List.split_length_fst {α} :
+    ∀ (xs : List α), xs.length ≤ 1 ∨ (split xs).fst.length < xs.length
+| [] => .inl (Nat.zero_le _)
+| [x] => .inl Nat.le.refl
+| [x, y] => .inr (Nat.lt.base _)
+| [x, y, z] => .inr (Nat.lt.base _)
+| x₁ :: x₂ :: x :: x' :: xs =>
+  have ih := split_length_fst (x :: x' :: xs);
+  by simp only [split, length]
+     apply Or.intro_right
+     apply Nat.succ_lt_succ
+     simp only [length, Nat.add] at ih
+     apply Nat.lt.step
+     cases ih with
+     | inl _ => contradiction
+     | inr h => apply h
+
+theorem List.split_length_snd {α} :
+    ∀ (xs : List α), xs = [] ∨ (split xs).snd.length < xs.length
+| [] => .inl rfl
+| [x] => .inr (Nat.lt.base _)
+| [x, y] => .inr (Nat.lt.base _)
+| x₁ :: x₂ :: x :: xs =>
+  have ih := split_length_snd (x :: xs);
+  by simp only [split, length]
+     apply Or.intro_right
+     apply Nat.succ_lt_succ
+     simp at ih
+     apply Nat.lt.step
+     apply ih
+
+theorem List.split_length_snd' {α} :
+    ∀ (xs : List α), (split xs).snd.length ≤ xs.length
+| [] => Nat.le.refl
+| [x] => Nat.le.step Nat.le.refl
+| x₁ :: x₂ :: xs =>
+  have ih := split_length_snd' xs;
+  by simp only [split, length]
+     apply Nat.le.step
+     apply Nat.succ_le_succ
+     apply ih
+
+def List.mergeWith {α} : (α → α → Ordering) → List α × List α → List α
+| _, ([], ys) => ys
+| _, (xs, []) => xs
+| cmp, (x :: xs, y :: ys) =>
+  have h1 : ys.length + (x :: xs).length <
+            (x :: xs).length + (y :: ys).length :=
+    by simp only [length]
+       rw [Nat.add_comm]
+       apply Nat.lt.base
+  have h2 : (y :: ys).length + xs.length <
+            (x :: xs).length + (y :: ys).length :=
+    by simp only [length]
+       rw [Nat.add_comm (length xs + 1)]
+       apply Nat.lt.base
+  match cmp x y with
+  | Ordering.gt => y :: mergeWith cmp (ys, x :: xs)
+  | _ => x :: mergeWith cmp (y :: ys, xs)
+termination_by cmp prd => prd.fst.length + prd.snd.length
+
+def List.mergeSortWith {α} : (α → α → Ordering) → List α → List α
+| _, [] => []
+| _, [x] => [x]
+| cmp, x₁ :: x₂ :: xs =>
+  have _ : (split (x₁::x₂::xs)).fst.length < (x₁::x₂::xs).length :=
+    match xs with
+    | [] => Nat.lt.base _
+    | [xs] => Nat.lt.base _
+    | y :: y' :: ys =>
+      match split_length_fst (y :: y' :: ys) with
+      | Or.inl _ => by contradiction
+      | Or.inr h =>
+        by simp only [length] at *
+           apply Nat.lt.step
+           apply Nat.succ_lt_succ
+           exact h
+
+   have _ : (split (x₁::x₂::xs)).snd.length < (x₁::x₂::xs).length :=
+    match xs with
+    | [] => Nat.lt.base _
+    | [xs] => Nat.lt.step (Nat.lt.base _)
+    | y :: y' :: ys =>
+      match split_length_snd (y :: y' :: ys) with
+      | Or.inl _ => by contradiction
+      | Or.inr h =>
+        by simp only [length] at *
+           apply Nat.lt.step
+           apply Nat.succ_lt_succ
+           exact h
+
+  let xs_split := split (x₁ :: x₂ :: xs)
+  mergeWith cmp (mergeSortWith cmp (xs_split.fst),
+                  mergeSortWith cmp (xs_split.snd))
+termination_by cmp xs => xs.length
+
+theorem List.length_mergeWith : ∀ (cmp : α → α → Ordering)
+                                   (xs ys : List α),
+  length (mergeWith cmp (xs, ys)) = length xs + length ys
+| cmp, [], ys => by simp only [mergeWith, length, Nat.zero_add]
+| cmp, x :: xs, [] => by simp only [mergeWith, length]
+| cmp, x :: xs, y :: ys =>
+have ih₁ := length_mergeWith cmp (y :: ys) xs
+have ih₂ := length_mergeWith cmp ys (x :: xs)
+by simp only [mergeWith]
+   cases cmp x y with
+   | lt =>
+     simp only
+     have h₁ : length (x :: mergeWith cmp (y :: ys, xs)) =
+               length (mergeWith cmp (y :: ys, xs)) + 1 := rfl
+     have h₂ : length (x :: xs) = length xs + 1 := rfl
+     rw [h₁, h₂, Nat.add_comm (length xs + 1), ←Nat.add_assoc]
+     apply congrArg (λ x => x + 1)
+     exact ih₁
+   | eq =>
+     simp only
+     have h₁ : length (x :: mergeWith cmp (y :: ys, xs)) =
+               length (mergeWith cmp (y :: ys, xs)) + 1 := rfl
+     have h₂ : length (x :: xs) = length xs + 1 := rfl
+     rw [h₁, h₂, Nat.add_comm (length xs + 1), ←Nat.add_assoc]
+     apply congrArg (λ x => x + 1)
+     exact ih₁
+   | gt =>
+     simp only [length]
+     simp only [length] at ih₂
+     rw [←Nat.add_assoc]
+     apply congrArg (λ x => x + 1)
+     rw [Nat.add_comm]
+     exact ih₂
+termination_by _ xs ys => xs.length + ys.length
+
+theorem List.length_split : ∀ (xs : List α),
+  length ((split xs).1) + length ((split xs).2) = length xs
+| [] => rfl
+| [x] => rfl
+| x :: y :: xs =>
+  have ih := length_split xs
+  by simp only [split, length]
+     rw [Nat.add_assoc (length xs),
+         Nat.add_assoc (length (split xs).1),
+         Nat.add_comm 1,
+         Nat.add_assoc (length (split xs).2),
+         ←Nat.add_assoc (length (split xs).1)]
+     apply congrArg (λ x => x + (1 + 1))
+     exact ih
+
+theorem List.length_mergeSortWith : ∀ (cmp : α → α → Ordering) (xs : List α),
+  length (mergeSortWith cmp xs) = length xs
+| _, [] => by simp only [mergeSortWith]
+| _, [x] => by simp only [mergeSortWith]
+| cmp, x :: y :: xs =>
+  have term₁ : Nat.succ (length (split xs).fst) <
+               Nat.succ (Nat.succ (length xs)) :=
+    Nat.succ_le_succ (Nat.succ_le_succ $ split_length_fst' xs)
+  have term₂ : Nat.succ (length (split xs).snd) <
+               Nat.succ (Nat.succ (length xs)) :=
+    Nat.succ_le_succ (Nat.succ_le_succ $ split_length_snd' xs)
+  have ih₁ := length_mergeSortWith cmp (x :: (split xs).1)
+  have ih₂ := length_mergeSortWith cmp (y :: (split xs).2)
+  -- TODO: we shouldn't need to do a "step" of length_split again here
+  by simp only [mergeSortWith, mergeWith, split, length_mergeWith, length]
+     rw [ih₁, ih₂]
+     simp only [length]
+     rw [Nat.add_assoc (length (split xs).1),
+         Nat.add_comm 1,
+         Nat.add_assoc (length (split xs).2),
+         ←Nat.add_assoc (length (split xs).1),
+         Nat.add_assoc (length xs)]
+     apply congrArg (λ x => x + (1 + 1))
+     apply length_split
+termination_by cmp xs => xs.length
