Table/BuiltinExtensions/List/Predicates.lean
@@ -1,0 +1,53 @@
+/-!
+Useful predicates on lists, including type-valued ones.
+-/
+
+-- List utilities
+inductive List.All {α} (p : α → Prop) : List α → Prop
+| vac      : All p []
+| cons {x xs} : p x → All p xs → All p (x::xs)
+
+inductive List.Unique {α} : List α → Prop
+  | nil : List.Unique []
+  | cons {x xs} : x ∉ xs → List.Unique xs → List.Unique (x :: xs)
+
+inductive List.UniqueT {α} : List α → Type _
+  | nil : List.UniqueT []
+  | cons {x xs} : x ∉ xs → List.UniqueT xs → List.UniqueT (x :: xs)
+
+inductive List.MemT {α : Type u} : α → List α → Type u
+| hd (x : α) (xs : List α) : List.MemT x (x :: xs)
+| tl (x : α) {y : α} {xs : List α} : List.MemT y xs → List.MemT y (x :: xs)
+
+infix:65 " <+ " => List.Sublist
+
+/-
+Below we include "structural" theorems about these predicates that don't rely on
+other list functions:
+-/
+
+theorem List.mem_of_memT {x : α} {xs : List α} : List.MemT x xs → List.Mem x xs
+| .hd _ _ => .head _
+| .tl _ h => .tail _ $ mem_of_memT h
+
+theorem List.neq_of_mem_not_mem {x y : α} {xs : List α} :
+  x ∈ xs → y ∉ xs → x ≠ y :=
+  λ hxs => mt (λ heq => heq ▸ hxs)
+
+theorem List.nil_singleton_of_all_eq_unique {xs : List α} :
+  (∀ x ∈ xs, ∀ y ∈ xs, x = y) →
+  Unique xs →
+  xs = [] ∨ ∃ x, xs = [x] := by
+  intro h hunique
+  cases hunique with
+  | nil => left; rfl
+  | @cons x xs hmem huniq =>
+    simp only [reduceCtorEq, cons.injEq, exists_and_right, exists_eq', true_and,
+               false_or]
+    cases xs with
+    | nil => rfl
+    | cons x' xs =>
+      have : x' ≠ x := λ heq => (heq ▸ hmem) (.head _)
+      have : x' = x := h x' (by simp only [mem_cons, or_true, true_or])
+                         x (by simp only [mem_cons, true_or])
+      contradiction
