Table/BuiltinExtensions/List/Sieve.lean
@@ -1,0 +1,150 @@
+import Table.BuiltinExtensions.List.Filtering
+
+/-!
+Contains `List.sieve` and associated lemmas.
+-/
+
+def List.sieve {α} : List Bool → List α → List α
+| [], xs => xs
+| _, [] => []
+| true :: bs, x :: xs => x :: sieve bs xs
+| false :: bs, _ :: xs => sieve bs xs
+
+theorem List.sieve_sublist : (bs : List Bool) → (xs : List α) →
+  Sublist (List.sieve bs xs) xs
+| [], [] => Sublist.slnil
+| [], x :: xs => List.sublist_self (x :: xs)
+| true :: bs, [] => Sublist.slnil
+| false :: bs, [] => Sublist.slnil
+| true :: bs, x :: xs => Sublist.cons₂ x (sieve_sublist bs xs)
+| false :: bs, x :: xs => Sublist.cons x (sieve_sublist bs xs)
+
+theorem List.sieve_removeAllEq : (bs : List Bool) → (xs : List α) →
+  length bs = length xs →
+    length (sieve bs xs) = length (removeAllEq bs [false])
+| [], [], h => rfl
+| b :: bs, [], h => by cases h
+| [], x :: xs, h => by cases h
+| true :: bs, x :: xs, h =>
+  have ih := sieve_removeAllEq bs xs (Nat.succ.inj h)
+  by rw [removeAllEq_singleton_hd_neq]
+     . simp only [length]
+       apply congrArg (λ x => x + 1)
+       exact ih
+     . apply Bool.noConfusion
+| false :: bs, x :: xs, h =>
+  have ih := sieve_removeAllEq bs xs (Nat.succ.inj h)
+  by rw [removeAllEq_singleton_hd_eq]
+     . simp only [length, sieve]
+       exact ih
+
+-- BEGIN lemmas for `selectColumns1_spec2`
+theorem List.sieve_mem_iff_true_unique :
+  ∀ {i} {xs : List α} {bs : List Bool} (pf1 pf2) (hu : List.Unique xs),
+  xs.get ⟨i, pf1⟩ ∈ bs.sieve xs ↔ bs.get ⟨i, pf2⟩ = true
+| 0, x :: xs, false :: bs, pf1, pf2, .cons hnmem hu' =>
+  Iff.intro
+    (λ hf =>
+      have not_mem_sieve_of_not_mem :=
+        mt (Sublist.mem.swap (sieve_sublist bs xs))
+      False.elim $ not_mem_sieve_of_not_mem hnmem hf)
+    (λ hb => nomatch hb)
+| 0, x :: xs, true :: bs, pf1, pf2, .cons hnmem hu' =>
+  Iff.intro
+    (λ _ => rfl)
+    (λ _ => List.Mem.head _)
+| .succ n, x :: xs, false :: bs, pf1, pf2, .cons hnmem hu' =>
+  have pf1' := Nat.lt_of_succ_lt_succ pf1
+  have pf2' := Nat.lt_of_succ_lt_succ pf2
+  Iff.intro
+    (λ hf => (sieve_mem_iff_true_unique pf1' pf2' hu').mp hf)
+    (λ hb => (sieve_mem_iff_true_unique pf1' pf2' hu').mpr hb)
+| .succ n, x :: xs, true :: bs, pf1, pf2, .cons hnmem hu' =>
+  Iff.intro
+    (λ hf => by
+      simp only [get, sieve] at *
+      apply Iff.mp
+      apply sieve_mem_iff_true_unique
+      . apply Nat.lt_of_succ_lt_succ pf1
+      . exact hu'
+      . exact List.get_mem_cons_of_head_not_mem_getee hf hnmem)
+    (λ hb => by
+      simp only [get, sieve] at *
+      apply Mem.tail
+      apply Iff.mpr
+      apply sieve_mem_iff_true_unique
+      . apply Nat.lt_of_succ_lt_succ pf2
+      . exact hu'
+      . exact hb)
+termination_by i xs bs pf1 pf2 hu => sizeOf xs + sizeOf bs
+
+theorem List.mem_map_sieve_of_mem_map {f : α → β} {x : α}
+  : ∀ {xs : List α} {bs : List Bool}, f x ∈ map f (sieve bs xs) → f x ∈ map f xs
+| [], [], h => nomatch h
+| x' :: xs, [], h => h
+| x' :: xs, false :: bs, h => Mem.tail _ $ mem_map_sieve_of_mem_map h
+| x' :: xs, true :: bs, h =>
+  match mem_cons.mp h with
+  | .inl heq => heq ▸ Mem.head _
+  | .inr hmem => Mem.tail _ $ mem_map_sieve_of_mem_map hmem
+
+theorem List.sieve_map_mem_iff_true_unique :
+  ∀ {i} {xs : List α} {bs : List Bool} (pf1 pf2) (f : α → β)
+    (hu : List.Unique (xs.map f)),
+  (xs.map f).get ⟨i, length_map xs f ▸ pf1⟩ ∈ (bs.sieve xs).map f
+  ↔ bs.get ⟨i, pf2⟩ = true := by
+  intro i xs bs pf1 pf2 f hu
+  apply Iff.intro
+  . intro hf
+    induction i generalizing xs bs with
+    | zero =>
+      match bs, xs, hu with
+      | b :: bs, x :: xs, .cons hnmem hu =>
+      cases b with
+      | true => simp only [get, sieve] at *
+      | false =>
+        simp only [get, sieve] at *
+        rw [Bool.false_eq_true]
+        exact mt mem_map_sieve_of_mem_map hnmem hf
+    | succ i ih =>
+      match bs, xs, hu with
+      | b :: bs, x :: xs, .cons hnmem hu =>
+      cases b with
+      | true =>
+        simp only [get, sieve, map] at *
+        apply ih
+        . exact hu
+        . apply get_mem_cons_of_head_not_mem_getee hf hnmem
+        . apply Nat.lt_of_succ_lt_succ pf1
+      | false =>
+        simp only [get, sieve, map] at *
+        apply ih
+        . exact hu
+        . exact hf
+        . apply Nat.lt_of_succ_lt_succ pf1
+  . intro hget
+    induction i generalizing xs bs with
+    | zero =>
+      match bs, xs with
+      | b :: bs, x :: xs =>
+      cases b with
+      | true => exact Mem.head _
+      | false => simp [get, map] at hget
+    | succ i ih =>
+      match bs, xs, hu with
+      | b :: bs, x :: xs, .cons hnmem hu =>
+      cases b with
+      | true =>
+        simp only [get, sieve, map] at *
+        apply Mem.tail
+        apply ih
+        . apply Nat.lt_of_succ_lt_succ pf1
+        . exact hu
+        . exact hget
+      | false =>
+        simp only [get, map, sieve] at *
+        apply ih
+        . apply Nat.lt_of_succ_lt_succ pf1
+        . exact hu
+        . exact hget
+-- END lemmas for `selectColumns1_spec2`
