Table/BuiltinExtensions/Logic.lean
@@ -1,0 +1,46 @@
+/-!
+Contains lemmas about existing logical operators and functions; also contains
+definitions for type-level logical operators.
+-/
+
+theorem not_or_distrib : ¬ (a ∨ b) ↔ ¬a ∧ ¬b :=
+Iff.intro
+(λ h => And.intro (λ ha => h (Or.intro_left _ ha))
+                  (λ hb => h (Or.intro_right _ hb)))
+(λ h => λ hneg =>
+  match hneg with
+  | Or.inl ha => h.left ha
+  | Or.inr hb => h.right hb)
+
+theorem not_not (p : Prop) : p → ¬¬p := λ hp hneg => hneg hp
+
+theorem Or.assoc : (P ∨ Q) ∨ R ↔ P ∨ Q ∨ R :=
+  Iff.intro (λ h => h.elim (λ hpq => hpq.elim Or.inl (Or.inr ∘ Or.inl))
+                           (Or.inr ∘ Or.inr))
+            (λ h => h.elim (Or.inl ∘ Or.inl)
+                           (λ hqr => hqr.elim (Or.inl ∘ Or.inr) Or.inr))
+
+theorem Iff.not_iff_not_of_iff : (p ↔ q) → (¬ p ↔ ¬ q) := λ hpq =>
+  Iff.intro (λ hnp hq => hnp $ hpq.mpr hq) (λ hnq hp => hnq $ hpq.mp hp)
+
+-- Basic fact about equality used in `removeHeaderHasCol'`
+theorem Eq.cast_distrib_fun {α} {x y : α} {σ τ : α → Type _}
+    (h : x = y) (f : ∀ {z}, τ z → σ z) (t : τ x) :
+    h ▸ (f t) = f (h ▸ t) :=
+  h.rec (Eq.refl (f t))
+
+def Injective (f : α → β) := ∀ a a', f a = f a' → a = a'
+
+def Function.swap (f : α → β → γ) : β → α → γ :=
+  λ b a => f a b
+
+-- Type-level negation for use with type-valued predicates
+def NotT (α : Type _) := α → Empty
+
+/- Equality type for pattern-matching workaround in proof of
+  `selectColumns2_spec3` -/
+inductive EqT : α → α → Type where
+  | refl (a : α) : EqT a a
+infix:50 " ≡ " => EqT
+
+def EqT.ofEq {a b : α} : a = b → a ≡ b := λ | .refl _ => .refl _
