Table/BuiltinExtensions/Numeric.lean
@@ -1,0 +1,30 @@
+/-!
+Lemmas about numeric types: `Nat` and `Int`.
+-/
+
+-- Based on `buffer.lt_aux_1` in Lean 3's `lib/lean/library/data/buffer.lean`
+theorem Nat.lt_of_lt_add_left {a b c : Nat} (h : a + c < b) : a < b :=
+Nat.lt_of_le_of_lt (Nat.le_add_right a c) h
+
+-- Reproducing `algebra/order/sub.lean` for Nats
+
+-- Based on `le_add_tsub` from Mathlib
+theorem Nat.le_add_sub {a b : Nat} : a ≤ b + (a - b) :=
+  Nat.sub_le_iff_le_add'.mp $ Nat.le_refl (a - b)
+
+theorem Nat.lt_of_sub_add {m k n : Nat} (hkm : k < m) (hn : n > 0) :
+    m - (k + n) < m - k :=
+  Nat.sub_lt_sub_left hkm (Nat.lt_add_of_pos_right hn)
+
+theorem Int.natAbs_of_nonneg_eq_toNat : ∀ z : Int, z ≥ 0 → z.natAbs = z.toNat
+  | ofNat n, h => rfl
+
+theorem Int.add_neg_eq_sub (m : Int) : ∀ n, n < 0 → m + n = m - n.natAbs
+  | negSucc n, h => rfl
+
+
+-- -- TODO: decide whether to use this or `Fin.instOfNat`
+-- instance (k : Nat) : OfNat (Fin k.succ) n :=
+--   if h : n < k.succ
+--   then ⟨n, h⟩
+--   else ⟨0, Nat.zero_lt_succ k⟩
