Table/Widgets.lean
@@ -16,13 +16,13 @@ instance {η nm τ} {xs : @Schema η}
          [τInst : ToHTML τ] [DecidableEq η] [rowInst : ToHTML (Row xs)]
     : ToHTML (Row ((nm, τ) :: xs)) where
   toHTML := λ (Row.cons cell d) =>
-                let s := match cell.toOption with
-                         | some v => "<td style=\"border:1px solid gray\">" ++ ToHTML.toHTML v ++ "</td>"
-                         | none   => "<td style=\"border:1px solid gray\"></td>";
-                let s_d := ToHTML.toHTML d
-                            |> String.drop (n := 4)
-                            |> String.dropRight (n := 5);
-                "<tr>" ++ s ++ s_d ++ "</tr>"
+    let curCell :=
+      match cell.toOption with
+      | some v => s!"<td style=\"border:1px solid gray\">{ToHTML.toHTML v}</td>"
+      | none   => "<td style=\"border:1px solid gray\"></td>";
+    let restOfRow :=
+      ToHTML.toHTML d |> String.drop (n := 4) |> String.dropRight (n := 5)
+    "<tr>" ++ curCell ++ restOfRow ++ "</tr>"
 
 instance {η} {schema : @Schema η}
          [ToHTML η] [DecidableEq η] [rowInst : ToHTML (Row schema)]
@@ -35,14 +35,16 @@ instance {η} {schema : @Schema η}
     ++ List.foldr (λ r acc => rowInst.toHTML r ++ acc) "" t.rows
     ++ "</tbody></table>"
 
-def mkTableWidget {η} [DecidableEq η] {schema : @Schema η} (t : Table schema) [htmlInst : ToHTML (Table schema)] :
-    UserWidgetDefinition where
-  name :=  "Display Table"
-  javascript :=  "
-    import * as React from 'react';
-    export default function(props) {
-      return React.createElement('div', {dangerouslySetInnerHTML: {__html: '" ++ ToHTML.toHTML t ++ "'}})
-    }"
+structure HTMLRendererWidgetProps where
+  html? : Option String
+  deriving Server.RpcEncodable
+
+@[widget_module] def htmlRendererWidget : Widget.Module where
+  javascript := "
+  import * as React from 'react';
+  export default function(props) {
+    return React.createElement('div', {dangerouslySetInnerHTML: {__html: props.html}})
+  }"
 
 -- TODO: in an ideal world, this wouldn't be necessary, but we keep this around
 -- to deal with reducibility issues
@@ -56,20 +58,16 @@ macro "html_inst" : tactic =>
     | infer_instance))
 
 syntax (name := tableWidgetCommand) "#table" term : command
--- TODO: this uses deprecated APIs
-@[command_elab tableWidgetCommand] private unsafe def elabTableWidget : Lean.Elab.Command.CommandElab :=
+
+@[command_elab tableWidgetCommand]
+private unsafe def elabTableWidget : Lean.Elab.Command.CommandElab :=
   open Lean Lean.Elab Command Term in λ
   | stx@`(#table $table:term) => do
-    let ns ← getCurrNamespace
-    let ident ← mkFreshIdent stx
-    let nm := ident.getId
-    let decl := Name.append ns nm
-
-    elabDeclaration (←
-      `(@[widget] def $ident := mkTableWidget ($table) (htmlInst := by html_inst))
-    )
-    let null_stx ← `(Json.null)
-    let props : Json ← runTermElabM fun _ =>
-      Term.evalTerm Json (mkConst ``Json) null_stx
-    Elab.Command.liftCoreM <| saveWidgetInfo decl props stx
+    let tableHTMLStx ← `(ToHTML.toHTML $table (self := by html_inst))
+    let tableHTML ← runTermElabM fun _ =>
+      evalTerm String (mkConst ``String) tableHTMLStx
+    let props : HTMLRendererWidgetProps := { html? := tableHTML }
+    let encodedProps := Server.RpcEncodable.rpcEncode props
+    Elab.Command.liftCoreM <|
+      savePanelWidgetInfo htmlRendererWidget.javascriptHash encodedProps stx
   | _ => throwUnsupportedSyntax
